More cleanup

LeanLion/QuickSort.lean
@@ -25,55 +25,48 @@ We define `smaller` and `larger` using `List.filter`. We need some theorems rela
 
 variable {α : Type}[LinearOrder α]
 
+@[grind]
 def smaller (pivot : α) (l : List α) : List α :=
   l.filter (fun x => x ≤  pivot)
 
+@[grind]
 def larger (pivot : α) (l : List α) : List α :=
-  l.filter (fun x => x > pivot)
+  l.filter (fun x => pivot < x)
 
 def quickSort : List α → List α
   | [] => []
   | pivot :: l =>
     have : (smaller pivot l).length < (pivot :: l).length := by
-      simp [List.length_cons]
-      apply Nat.succ_le_succ
-      apply List.length_filter_le
+      grind
     have : (larger pivot l).length < (pivot :: l).length := by
-      simp [List.length_cons]
-      apply Nat.succ_le_succ
-      apply List.length_filter_le
+      grind
     (quickSort (smaller pivot l)) ++ pivot :: (quickSort (larger pivot l))
 termination_by l => l.length
 
-@[simp]
+
+@[simp, grind]
 theorem quickSort_nil : quickSort ([] : List α) = [] := by
   simp [quickSort]
 
-@[simp]
+@[simp, grind]
 theorem quickSort_cons (pivot : α) (l : List α) :
     quickSort (pivot :: l) = (quickSort (smaller pivot l)) ++
     pivot :: (quickSort (larger pivot l)) := by
   simp [quickSort]
 
-theorem mem_iff_below_or_above_pivot (pivot : α) (l : List α)(x : α) :
+@[grind]
+theorem mem_iff_below_or_above_pivot (pivot : α)
+  (l : List α)(x : α) :
     x ∈ l ↔ x ∈ smaller pivot l ∨ x ∈ larger pivot l := by
   apply Iff.intro
   · intro h
     by_cases h' : x ≤ pivot
     · left
-      rw [smaller, List.mem_filter]
-      simp [h, h']
+      grind
     · right
-      rw [larger, List.mem_filter]
-      simp [h, lt_of_not_ge h']
+      grind [lt_iff_not_ge]
   · intro h
-    cases h with
-    | inl h =>
-      rw [smaller, List.mem_filter] at h
-      exact h.left
-    | inr h =>
-      rw [larger, List.mem_filter] at h
-      exact h.left
+    grind
 
 theorem mem_iff_mem_quickSort (l: List α)(x : α) :
     x ∈ l ↔ x ∈ quickSort l := by
@@ -81,20 +74,13 @@ theorem mem_iff_mem_quickSort (l: List α)(x : α) :
   | nil =>
     simp
   | cons pivot l =>
-    simp
-    rw [mem_iff_below_or_above_pivot pivot]
     have : (smaller pivot l).length < (pivot :: l).length := by
-      simp [List.length_cons]
-      apply Nat.succ_le_succ
-      apply List.length_filter_le
+      grind
     have : (larger pivot l).length < (pivot :: l).length := by
-      simp [List.length_cons]
-      apply Nat.succ_le_succ
-      apply List.length_filter_le
+      grind
     have ihb := mem_iff_mem_quickSort (smaller pivot l)
     have iha := mem_iff_mem_quickSort (larger pivot l)
-    rw [← ihb, ← iha]
-    tauto
+    grind
 termination_by l.length
 
 inductive Sorted : List α → Prop
@@ -102,6 +88,92 @@ inductive Sorted : List α → Prop
   | singleton (x : α) : Sorted [x]
   | step (x y : α) (l : List α) (hxy: x ≤ y)
       (tail_sorted: Sorted (y :: l)) : Sorted (x :: y :: l)
+
+@[grind]
+theorem head_le_of_sorted  (a: α) (l : List α) :
+  Sorted (a :: l) → ∀ x ∈ l, a ≤ x := by
+  intro h
+  match h with
+  | Sorted.singleton .. => simp
+  | Sorted.step x y l hxy tail_sorted =>
+    intro z hz
+    simp at hz
+    cases hz
+    · grind
+    · have ih := head_le_of_sorted y l tail_sorted
+      trans y
+      · assumption
+      · grind
+
+theorem cons_sorted (l : List α) :  Sorted l → (a : α) →
+  (∀ y ∈ l, a ≤ y) → Sorted (a :: l)  := by
+  intro h₁
+  induction h₁ with
+  | nil =>
+    intro a h₀
+    apply Sorted.singleton
+  | singleton x =>
+    intro a h₀
+    simp at h₀
+    apply Sorted.step a x
+    · assumption
+    · apply Sorted.singleton
+  | step x y l hxy tail_sorted ih =>
+    intro a h₀
+    simp at h₀
+    rcases h₀ with ⟨h₁, h₂, h₃⟩
+    apply Sorted.step a x (y :: l)
+    · assumption
+    · apply ih
+      simp [hxy]
+      intro z hz
+      trans y
+      · assumption
+      · grind
+
+theorem sorted_sandwitch (l₁ : List α) (h₁ : Sorted l₁)
+    (l₂ : List α) (h₂ : Sorted l₂)
+    (bound : α)
+    (h_bound₁ : ∀ x ∈ l₁, x ≤ bound)
+    (h_bound₂ : ∀ x ∈ l₂, bound ≤ x) :
+    Sorted (l₁ ++ bound :: l₂) := by
+    induction h₁ with
+    | nil =>
+      simp only [List.nil_append]
+      apply cons_sorted l₂ h₂ bound h_bound₂
+    | singleton x =>
+      simp only [List.cons_append, List.nil_append]
+      apply Sorted.step x bound l₂
+      · grind
+      · apply cons_sorted l₂ h₂ bound h_bound₂
+    | step x y l hxy tail_sorted ih =>
+      simp only [List.cons_append]
+      apply Sorted.step x y (l ++ bound :: l₂) hxy
+      grind
+
+theorem quickSort_sorted (l : List α) : Sorted (quickSort l) := by
+  cases l with
+  | nil =>
+    simp [quickSort_nil]
+    apply Sorted.nil
+  | cons pivot l =>
+    rw [quickSort_cons]
+    have : (smaller pivot l).length < (pivot :: l).length := by
+      grind
+    have : (larger pivot l).length < (pivot :: l).length := by
+      grind
+    apply sorted_sandwitch
+    · apply quickSort_sorted (smaller pivot l)
+    · apply quickSort_sorted (larger pivot l)
+    · intro x
+      rw [← mem_iff_mem_quickSort]
+      grind
+    · intro x
+      rw [← mem_iff_mem_quickSort]
+      grind [le_of_lt]
+termination_by l.length
+
+-- Older code
 
 theorem append_sorted (bound: α)(l₁ l₂ : List α) :
   (∀ x ∈ l₁, x ≤ bound) → (∀ x ∈ l₂, bound ≤  x) → Sorted l₁ → Sorted l₂ → Sorted (l₁ ++ l₂) := by
@@ -137,7 +209,7 @@ theorem append_sorted (bound: α)(l₁ l₂ : List α) :
       · apply h₁.right.right
     · exact s₂
 
-theorem quickSort_sorted (l : List α) : Sorted (quickSort l) := by
+theorem quickSort_sorted' (l : List α) : Sorted (quickSort l) := by
   cases l with
   | nil =>
     simp [quickSort_nil]
@@ -152,8 +224,8 @@ theorem quickSort_sorted (l : List α) : Sorted (quickSort l) := by
       simp [List.length_cons]
       apply Nat.succ_le_succ
       apply List.length_filter_le
-    let ihb := quickSort_sorted (smaller pivot l)
-    let iha := quickSort_sorted (larger pivot l)
+    let ihb := quickSort_sorted' (smaller pivot l)
+    let iha := quickSort_sorted' (larger pivot l)
     apply append_sorted pivot
     · intro x
       rw [← mem_iff_mem_quickSort]
@@ -181,3 +253,18 @@ theorem quickSort_sorted (l : List α) : Sorted (quickSort l) := by
       · apply Sorted.singleton
       · assumption
 termination_by l.length
+
+
+set_option pp.all true in
+#print quickSort
+
+/-
+{α : Sort u} →
+  {C : α → Sort v} → {r : α → α → Prop} → WellFounded r → ((x : α) → ((y : α) → r y x → C y) → C x) → (x : α) → C x
+-/
+#check WellFounded.fix
+
+/- {α : Sort u} →
+  {r : α → α → Prop} → WellFounded r → {C : α → Sort v} → (a : α) → ((x : α) → ((y : α) → r y x → C y) → C x) → C a
+-/
+#check WellFounded.recursion
